\documentclass{article}

\usepackage{fancyhdr}
\pagestyle{fancy}
\lhead{Ruicheng Wu}
\rhead{07/11/2017}
\chead{Homework 6}

\begin{document}
1.
$E(n) = Z(n)+ O(n) + T(n)$,E : all ternary sequence; Z ： sequence ends with 0 ; O ： sequence ends with 1;T ： sequence ends with 2;
$$E(n) = Z(n)+ O(n) + T(n)$$
$$Z(n) = T(n-1)$$
$$O(n) = T(n-1)$$
$$T(n) = Z(n-1)+ O(n-1) + T(n-1) $$
now substitute each term with RHS terms.
$$E(n) = Z(n-1)+ O(n-1) + T(n-1)+ 2*T(n-1)$$
$$= E(n-1)+ 2*E(n-2)$$.Thus proves the recurrence relation is true.\\

Given, $h_x-h_{x-1}-2h_{x-2}=0$.
\\Assume there is 

$h(x) = h_0+h_1x+h_2x^2+h_3x^3...+h_nx^n$

$-xh(x) = 0-h_0x-h_1x^2-h_2x^3-h_3x^4...-h_{n-1}x^n$

$-2x^2h(x) = 0+0-2h_0x^2-2h_1x^3-2h_2x^4-2h_3x^5...-2h_{n-2}x^n$

Add them together:

$(1-x-2x^2)h(x)=h_0+(h_1-h_0)x$

$h(x)=\frac{1+2x}{(1-x-2x^2)}=\frac{c_1}{-2x+1}+\frac{c_2}{x+1}$

Solve for $c_1,c_2$:

$(c_1-2c_2)x+(c_1+c_2)=2x+1$

$c_1+c_2=1$

$c_1-2c_2=2$

$c_1=\frac{4}{3}$,$c_2=-\frac{1}{3}$

Now plug in $c_1,c_2$:

$h(x)=\frac{4}{3}*\frac{1}{-2x+1}-\frac{1}{3}*\frac{1}{x+1}$

convert into summation:

$$\frac{4}{3}*\sum_{k=0}2^kx^k-\frac{1}{3}*\sum(-1)^kx^k$$

$$\sum_{k=0}[\frac{4}{3}*2^k+(-\frac{1}{3})*(-1)^k]x^k$$

Now we obtain the part for $a_n$,which is $[\frac{4}{3}*2^k+(-\frac{1}{3})*(-1)^k]$

2.

Guessing method:

Since the particular part is $n$, we guess solution to it is :
$an+b$,plug in:

$an+b=2(a(n-1)+b)+n$

$0=(a+1)n-(2a-b)$

solve for a,b ： $a = -1,b=-2$

Now $-n-2$ is one solution to recurrence relation(Not the initial condition!),now we add a solution to the homogenous part, which is $c2^n$.By setting up the initial condition,we can solve for $c$:

$h_0=-(0)-2+c2^{(0)}=1$,$c=3$

So $h_n = -n-2+3*2^n$

Generating function:we have $h_n-2h_{n-1}-n=0$

$h(x) = h_0+h_1x+h_2x^2+h_3x^3...+h_nx^n$

$-2xh(x) = 0-2h_0x-2h_1x^2-2h_2x^3...-2h_{n-1}x^n$

$-\sum_{n>=0}n*x^n = 0-1x-2x^2-3x^3...-nx^n$

By adding these equations together

$$(1-2x)h(x)-\sum_{n>=0}n*x^n = h_0 = 1$$

$$h(x)=\frac{1+\frac{x}{{(1-x)}^2}}{(1-2x)}=\frac{x^2-x+1}{(1-x)^2*(1-2x)}$$

$$=\frac{c_1}{(1-x)}+\frac{c_2}{(1-x)^2}+\frac{c_3}{(1-2x)}$$

$$=c_1+c_2+c_3-(3c_1+2c_2+2c_3)x+(2c_1+c_3)x^2$$

$$c_1+c_2+c_3=1$$
$$3c_1+2c_2+2c_3=1$$
$$2c_1+c_3=1$$

set up matrix and solve them,$c_1=-1,c_2=-1,c_3=3$.

$$h(x)=\frac{-1}{(1-x)}+\frac{{-1}}{(1-x)^2}+\frac{3}{(1-2x)}$$

$$=\sum_n(-1)*x^n+\sum_n{-1}*C(n+2-1,n)x^n++\sum_n3*2^nx^n$$
$$=\sum_n(-1-n-1+3*2^n)x^n$$
$$=\sum_n(-n-2+3*2^n)x^n$$

So,$h_n = -n-2+3*2^n $.

Since the g.f method produce the exact same answer as guessing method, they prove each other are correct answers amazingly !


3.
Using Guessing method:

Since the particular part is $2n$, we guess solution to it is :
$an+b$,plug in:

$an+b=6(a(n-1)+b)-9(a(n-2)+b)+2n$

$(4a − 2)n + (4b − 12a) = 0$

so a = $\frac{1}{2}$,and b =$\frac{3}{2}$


Now $\frac{1}{2}n+\frac{3}{2}$ is one solution to recurrence relation(Not the initial condition!),now we add a solution to the homogenous part, which is $c_13^n + c_2n3^n$.By setting up the initial condition,we can solve for $c_1,c_2$:

$h_0 = c_13^0 + c_2*0*3^0 + \frac{1}{2}*0+\frac{3}{2}$

$h_1 = c_13^1 + c_2*1*3^1 + \frac{1}{2}*1+\frac{3}{2}$

solve for $c_1,c_2$:

$c_1=-\frac{1}{2}$,$c_2=-\frac{1}{6}$

$h(x)=-\frac{1}{2}*3^n-\frac{1}{6}n*3^n+\frac{1}{2}n+\frac{3}{2}$




\end{document}